Move dead code elimination to own subdir

theories/DeadCodeElimination/DCE.v
@@ -14,7 +14,7 @@ Notation "'co_ra' x" := (snd x) (at level 10, only parsing).
 Hint Resolve reachability_SC_S correct.
 
 (*
-Definition DCVE i (s:IL.stmt) (ra:ann (⦃var⦄ * ⦃var⦄)) : stmt * ann ⦃var⦄ * ann (⦃var⦄ * ⦃var⦄) :=
+Definition DCE i (s:IL.stmt) (ra:ann (⦃var⦄ * ⦃var⦄)) : stmt * ann ⦃var⦄ * ann (⦃var⦄ * ⦃var⦄) :=
   let uc := reachabilityAnalysis s in
   let s_uce := UCE.compile nil s uc in
   let ra_uce := UCE.compile_renamedApart s ra uc in
@@ -24,14 +24,14 @@ Definition DCVE i (s:IL.stmt) (ra:ann (⦃var⦄ * ⦃var⦄)) : stmt * ann ⦃v
   (s_dve, DVE.compile_live s_uce tlv ∅, ra_dve).
 *)
 
-Definition DCVE i (s:IL.stmt) : stmt * ann ⦃var⦄ :=
+Definition DCE i (s:IL.stmt) : stmt * ann ⦃var⦄ :=
   let uc := reachabilityAnalysis s in
   let s_uce := UCE.compile nil s uc in
   let tlv := LivenessAnalysis.livenessAnalysis i s_uce in
   let s_dve := DVE.compile nil s_uce tlv in
   (s_dve, DVE.compile_live s_uce tlv ∅).
 
-Definition DCVEra i (s:IL.stmt) (ra:ann (⦃var⦄ * ⦃var⦄)) : ann (⦃var⦄ * ⦃var⦄) :=
+Definition DCEra i (s:IL.stmt) (ra:ann (⦃var⦄ * ⦃var⦄)) : ann (⦃var⦄ * ⦃var⦄) :=
   let uc := reachabilityAnalysis s in
   let s_uce := UCE.compile nil s uc in
   let ra_uce := UCE.compile_renamedApart s ra uc in
@@ -40,7 +40,7 @@ Definition DCVEra i (s:IL.stmt) (ra:ann (⦃var⦄ * ⦃var⦄)) : ann (⦃var�
   ra_dve.
 
 
-Lemma DCVE_true_live_sound i s (PM:LabelsDefined.paramsMatch s nil)
+Lemma DCE_true_live_sound i s (PM:LabelsDefined.paramsMatch s nil)
   : true_live_sound i nil nil (UCE.compile nil s (reachabilityAnalysis s))
                     (LivenessAnalysis.livenessAnalysis i (UCE.compile nil s (reachabilityAnalysis s))).
 Proof.
@@ -49,37 +49,37 @@ Proof.
     + eapply reachabilityAnalysis_getAnn.
 Qed.
 
-Hint Resolve DCVE_true_live_sound.
+Hint Resolve DCE_true_live_sound.
 
-Lemma DCVE_UCE_params_match s (PM:LabelsDefined.paramsMatch s nil)
+Lemma DCE_UCE_params_match s (PM:LabelsDefined.paramsMatch s nil)
   : paramsMatch (UCE.compile nil s (reachabilityAnalysis s)) nil.
 Proof.
   eapply (@UCE.UCE_paramsMatch nil nil); eauto.
   eapply reachabilityAnalysis_getAnn.
 Qed.
 
-Hint Resolve DCVE_UCE_params_match.
+Hint Resolve DCE_UCE_params_match.
 
-Lemma DCVE_live i (ili:IL.stmt) (PM:LabelsDefined.paramsMatch ili nil)
-  : Liveness.live_sound i nil nil (fst (DCVE i ili)) (snd (DCVE i ili)).
+Lemma DCE_live i (ili:IL.stmt) (PM:LabelsDefined.paramsMatch ili nil)
+  : Liveness.live_sound i nil nil (fst (DCE i ili)) (snd (DCE i ili)).
 Proof.
-  unfold DCVE. simpl.
+  unfold DCE. simpl.
   eapply (@DVE.dve_live _ nil nil).
   eapply @LivenessAnalysisCorrect.correct; eauto.
 Qed.
 
-Lemma DCVE_UCE_renamedApart s ra (PM:LabelsDefined.paramsMatch s nil) (RA:renamedApart s ra)
+Lemma DCE_UCE_renamedApart s ra (PM:LabelsDefined.paramsMatch s nil) (RA:renamedApart s ra)
   :  renamedApart (UCE.compile nil s (reachabilityAnalysis s))
                   (UCE.compile_renamedApart s ra (reachabilityAnalysis s)).
 Proof.
   eapply UCE.UCE_renamedApart; eauto.
 Qed.
 
-Hint Resolve DCVE_UCE_renamedApart.
+Hint Resolve DCE_UCE_renamedApart.
 
-Lemma DCVE_noUC b i ili (PM:LabelsDefined.paramsMatch ili nil)
+Lemma DCE_noUC b i ili (PM:LabelsDefined.paramsMatch ili nil)
   : LabelsDefined.noUnreachableCode (LabelsDefined.isCalled b)
-                                    (fst (DCVE i ili)).
+                                    (fst (DCE i ili)).
 Proof.
   intros. subst. simpl.
   eapply LabelsDefined.noUnreachableCode_mono.
@@ -90,8 +90,8 @@ Proof.
   - intros; eapply LabelsDefined.trueIsCalled_isCalled; eauto.
 Qed.
 
-Lemma DCVE_occurVars i s (PM:LabelsDefined.paramsMatch s nil)
-  : getAnn (snd (DCVE i s)) ⊆ occurVars s.
+Lemma DCE_occurVars i s (PM:LabelsDefined.paramsMatch s nil)
+  : getAnn (snd (DCE i s)) ⊆ occurVars s.
 Proof.
   simpl.
   rewrite DVE.compile_live_incl_empty; eauto.
@@ -99,11 +99,11 @@ Proof.
   eapply UCE.compile_occurVars.
 Qed.
 
-Lemma DCVE_correct_I (ili:IL.stmt) (E:onv val)
+Lemma DCE_correct_I (ili:IL.stmt) (E:onv val)
   (PM:LabelsDefined.paramsMatch ili nil)
-  : sim I.state I.state bot3 Sim (nil, E, ili) (nil, E, fst (DCVE Liveness.Imperative ili)).
+  : sim I.state I.state bot3 Sim (nil, E, ili) (nil, E, fst (DCE Liveness.Imperative ili)).
 Proof.
-  intros. subst. unfold DCVE.
+  intros. subst. unfold DCE.
   simpl in *.
   assert (reachability cop2bool SoundAndComplete nil ili
                                            (reachabilityAnalysis ili)). {
@@ -127,12 +127,12 @@ Proof.
   eapply DVE.I.sim_DVE; [ reflexivity | eapply LivenessAnalysisCorrect.correct; eauto ].
 Qed.
 
-Lemma DCVE_correct_F (ilf:IL.stmt) (E:onv val)
+Lemma DCE_correct_F (ilf:IL.stmt) (E:onv val)
   (PM:LabelsDefined.paramsMatch ilf nil)
   : defined_on (IL.occurVars ilf) E
-    -> sim F.state F.state bot3 Sim (nil, E, ilf) (nil, E, fst (DCVE Liveness.Functional ilf)).
+    -> sim F.state F.state bot3 Sim (nil, E, ilf) (nil, E, fst (DCE Liveness.Functional ilf)).
 Proof.
-  intros. subst. unfold DCVE.
+  intros. subst. unfold DCE.
   simpl in *.
   assert (reachability cop2bool SoundAndComplete nil ilf
                                            (reachabilityAnalysis ilf)). {
@@ -163,9 +163,9 @@ Definition compile_renamedApart i s ra :=
                            ra'
                            (fst (getAnn ra')).
 
-Lemma DCVE_renamedApart i s ra (PM:LabelsDefined.paramsMatch s nil)
+Lemma DCE_renamedApart i s ra (PM:LabelsDefined.paramsMatch s nil)
   : renamedApart s ra
-    -> renamedApart (fst (DCVE i s)) (DCVEra i s ra).
+    -> renamedApart (fst (DCE i s)) (DCEra i s ra).
 Proof.
   intros. simpl.
   exploit (@LivenessAnalysisCorrect.correct i); eauto.
@@ -186,7 +186,7 @@ Proof.
 Qed.
 
 
-Lemma DCVE_true_live_sound_F i s ra (PM:LabelsDefined.paramsMatch s nil) (RA:renamedApart s ra)
+Lemma DCE_true_live_sound_F i s ra (PM:LabelsDefined.paramsMatch s nil) (RA:renamedApart s ra)
   : true_live_sound Functional nil nil (UCE.compile nil s (reachabilityAnalysis s))
                     (LivenessAnalysis.livenessAnalysis i (UCE.compile nil s (reachabilityAnalysis s))).
 Proof.
@@ -201,15 +201,15 @@ Proof.
   - isabsurd.
 Qed.
 
-Lemma DCVE_live_incl i s ra (RA:renamedApart s ra) (PM:LabelsDefined.paramsMatch s nil)
+Lemma DCE_live_incl i s ra (RA:renamedApart s ra) (PM:LabelsDefined.paramsMatch s nil)
   : ann_R (fun (x : ⦃var⦄) (y : ⦃var⦄ * ⦃var⦄) => x ⊆ fst y)
-          (snd (DCVE i s)) (DCVEra i s ra).
+          (snd (DCE i s)) (DCEra i s ra).
 Proof.
-  unfold DCVE; simpl.
+  unfold DCE; simpl.
   eapply DVE.DVE_live_incl.
   - instantiate (1:=Functional). eauto.
   - eapply UCE.UCE_renamedApart; eauto.
-  - eapply DCVE_true_live_sound_F; eauto.
+  - eapply DCE_true_live_sound_F; eauto.
   - eapply LivenessAnalysisCorrect.livenessAnalysis_renamedApart_incl; eauto.
   - exploit (@LivenessAnalysisCorrect.livenessAnalysis_renamedApart_incl
                i (UCE.compile nil s (reachabilityAnalysis s))); eauto.
@@ -218,47 +218,47 @@ Proof.
   - eauto with cset.
 Qed.
 
-Lemma DCVE_paramsMatch i s (PM:LabelsDefined.paramsMatch s nil)
-  : LabelsDefined.paramsMatch (fst (DCVE i s)) nil.
+Lemma DCE_paramsMatch i s (PM:LabelsDefined.paramsMatch s nil)
+  : LabelsDefined.paramsMatch (fst (DCE i s)) nil.
 Proof.
-  unfold DCVE; simpl.
+  unfold DCE; simpl.
   exploit (@DVE.DVE_paramsMatch i nil nil); eauto.
 Qed.
 
-Lemma DCVE_app_expfree i s
+Lemma DCE_app_expfree i s
       (AEF:app_expfree s)
-  : app_expfree (fst (DCVE i s)).
+  : app_expfree (fst (DCE i s)).
 Proof.
   simpl.
   eapply DVE.DVE_app_expfree.
   eapply UCE.UCE_app_expfree; eauto.
 Qed.
 
-Lemma DCVE_ra_fst s ra
+Lemma DCE_ra_fst s ra
       (PM:LabelsDefined.paramsMatch s nil) (RA:renamedApart s ra)
-  : fst (getAnn (DCVEra Liveness.Imperative s ra))
+  : fst (getAnn (DCEra Liveness.Imperative s ra))
         [=] fst (getAnn ra).
 Proof.
-  unfold DCVEra.
+  unfold DCEra.
   rewrite DVE.fst_getAnn_renamedApart'; eauto.
   exploit UCE.compile_renamedApart_pes; eauto.
   + rewrite H. reflexivity.
 Qed.
 
-Lemma DCVE_ra_snd s ra
+Lemma DCE_ra_snd s ra
       (PM:LabelsDefined.paramsMatch s nil) (RA:renamedApart s ra)
-  : snd (getAnn (DCVEra Liveness.Imperative s ra))
+  : snd (getAnn (DCEra Liveness.Imperative s ra))
         ⊆ snd (getAnn ra).
 Proof.
-  unfold DCVEra.
+  unfold DCEra.
   rewrite DVE.snd_getAnn_renamedApart; eauto.
   exploit UCE.compile_renamedApart_pes; eauto.
   + rewrite H. reflexivity.
 Qed.
 
-Lemma DCVE_var_P i (P:var -> Prop) (s:stmt) (PM:LabelsDefined.paramsMatch s nil)
+Lemma DCE_var_P i (P:var -> Prop) (s:stmt) (PM:LabelsDefined.paramsMatch s nil)
   (VP:var_P P s)
-  : var_P P (fst (DCVE i s)).
+  : var_P P (fst (DCE i s)).
 Proof.
   simpl.
   eapply (@DVE.DVE_var_P i _ nil nil); eauto.
